



# ***Data Structures and Algorithms***

## ***Solving Recurrence Relations***

Chris Brooks

Department of Computer Science  
University of San Francisco

## ***4-0: Algorithm Analysis***

```
for (i=1; i<=n*n; i++)  
    for (j=0; j<i; j++)  
        sum++;
```

## 4-1: Algorithm Analysis

<code>for (i=1; i&lt;=n*n; i++)</code>	Executed $n*n$ times
<code>    for (j=0; j&lt;i; j++)</code>	Executed $\leq n*n$ times
<code>        sum++;</code>	$O(1)$

Running Time:  $O(n^4)$

But can we get a tighter bound?

## 4-2: Algorithm Analysis

```
for (i=1; i<=n*n; i++)  
    for (j=0; j<i; j++)  
        sum++;
```

Exact # of times `sum++` is executed:

$$\begin{aligned}\sum_{i=1}^{n^2} i &= \frac{n^2(n^2 + 1)}{2} \\ &= \frac{n^4 + n^2}{2} \\ &\in \Theta(n^4)\end{aligned}$$

## 4-3: *Recursive Functions*

```
long power(long x, long n)
    if (n == 0)
        return 1;
    else
        return x * power(x, n-1);
```

How many times is this executed?

## 4-4: *Recurrence Relations*

$T(n)$  = Time required to solve a problem of size  $n$

Recurrence relations are used to determine the running time of recursive programs – recurrence relations themselves are recursive

$T(0)$  = time to solve problem of size 0  
– Base Case

$T(n)$  = time to solve problem of size  $n$   
– Recursive Case

## 4-5: *Recurrence Relations*

```
long power(long x, long n)
    if (n == 0)
        return 1;
    else
        return x * power(x, n-1);
```

$T(0) = c_1$  for some constant  $c_1$

$T(n) = c_2 + T(n - 1)$  for some constant  $c_2$

## ***4-6: Solving Recurrence Relations***

$$T(0) = c_1$$

$$T(n) = T(n - 1) + c_2$$

If we knew  $T(n - 1)$ , we could solve  $T(n)$ .

$$T(n) = T(n - 1) + c_2$$



## 4-7: Solving Recurrence Relations

$$T(0) = c_1$$

$$T(n) = T(n - 1) + c_2$$

If we knew  $T(n - 1)$ , we could solve  $T(n)$ .

$$\begin{aligned} T(n) &= T(n - 1) + c_2 & T(n - 1) &= T(n - 2) + c_2 \\ &= T(n - 2) + c_2 + c_2 \\ &= T(n - 2) + 2c_2 \end{aligned}$$

## 4-8: Solving Recurrence Relations

$$T(0) = c_1$$

$$T(n) = T(n - 1) + c_2$$

If we knew  $T(n - 1)$ , we could solve  $T(n)$ .

$$\begin{aligned} T(n) &= T(n - 1) + c_2 & T(n - 1) &= T(n - 2) + c_2 \\ &= T(n - 2) + c_2 + c_2 \\ &= T(n - 2) + 2c_2 & T(n - 2) &= T(n - 3) + c_2 \\ &= T(n - 3) + c_2 + 2c_2 \\ &= T(n - 3) + 3c_2 \end{aligned}$$

## 4-9: Solving Recurrence Relations

$$T(0) = c_1$$

$$T(n) = T(n - 1) + c_2$$

If we knew  $T(n - 1)$ , we could solve  $T(n)$ .

$$\begin{aligned} T(n) &= T(n - 1) + c_2 & T(n - 1) &= T(n - 2) + c_2 \\ &= T(n - 2) + c_2 + c_2 \\ &= T(n - 2) + 2c_2 & T(n - 2) &= T(n - 3) + c_2 \\ &= T(n - 3) + c_2 + 2c_2 \\ &= T(n - 3) + 3c_2 & T(n - 3) &= T(n - 4) + c_2 \\ &= T(n - 4) + 4c_2 \end{aligned}$$

## 4-10: Solving Recurrence Relations

$$T(0) = c_1$$

$$T(n) = T(n - 1) + c_2$$

If we knew  $T(n - 1)$ , we could solve  $T(n)$ .

$$\begin{aligned} T(n) &= T(n - 1) + c_2 & T(n - 1) &= T(n - 2) + c_2 \\ &= T(n - 2) + c_2 + c_2 \\ &= T(n - 2) + 2c_2 & T(n - 2) &= T(n - 3) + c_2 \\ &= T(n - 3) + c_2 + 2c_2 \\ &= T(n - 3) + 3c_2 & T(n - 3) &= T(n - 4) + c_2 \\ &= T(n - 4) + 4c_2 \\ &= \dots \\ &= T(n - k) + kc_2 \end{aligned}$$

## 4-11: Solving Recurrence Relations

$$T(0) = c_1$$

$$T(n) = T(n - k) + k * c_2 \quad \text{for all } k$$

If we set  $k = n$ , we have:

$$\begin{aligned} T(n) &= T(n - n) + nc_2 \\ &= T(0) + nc_2 \\ &= c_1 + nc_2 \\ &\in \Theta(n) \end{aligned}$$

## 4-12: *Building a Better* Power

Can we avoid making a linear number of function calls?

```
long power(long x, long n)
    if (n==0) return 1;
    if (n==1) return x;
    if ((n % 2) == 0)
        return power(x*x, n/2);
    else
        return power(x*x, n/2) * x;
```

## 4-13: *Building a Better* Power

```
long power(long x, long n)
    if (n==0) return 1;
    if (n==1) return x;
    if ((n % 2) == 0)
        return power(x*x, n/2);
    else
        return power(x*x, n/2) * x;
```

$$T(0) = c_1$$

$$T(1) = c_2$$

$$T(n) = T(n/2) + c_3$$

(Assume n is a power of 2)

## ***4-14: Solving Recurrence Relations***

$$T(n) = T(n/2) + c_3$$



## ***4-15: Solving Recurrence Relations***

$$\begin{aligned} T(n) &= T(n/2) + c_3 & T(n/2) &= T(n/4) + c_3 \\ &= T(n/4) + c_3 + c_3 \\ &= T(n/4) + 2c_3 \end{aligned}$$

## 4-16: Solving Recurrence Relations

$$\begin{aligned}T(n) &= T(n/2) + c_3 \\&= T(n/4) + c_3 + c_3 \\&= T(n/4) + 2c_3 \\&= T(n/8) + c_3 + 2c_3 \\&= T(n/8) + 3c_3\end{aligned}$$

$$T(n/2) = T(n/4) + c_3$$

$$T(n/4) = T(n/8) + c_3$$

## 4-17: Solving Recurrence Relations

$$\begin{aligned}T(n) &= T(n/2) + c_3 \\&= T(n/4) + c_3 + c_3 \\&= T(n/4) + 2c_3 \\&= T(n/8) + c_3 + 2c_3 \\&= T(n/8) + 3c_3 \\&= T(n/16) + c_3 + 3c_3 \\&= T(n/16) + 4c_3\end{aligned}$$

$$T(n/2) = T(n/4) + c_3$$

$$T(n/4) = T(n/8) + c_3$$

$$T(n/8) = T(n/16) + c_3$$

## 4-18: Solving Recurrence Relations

$$\begin{aligned}T(n) &= T(n/2) + c_3 \\&= T(n/4) + c_3 + c_3 \\&= T(n/4)2c_3 \\&= T(n/8) + c_3 + 2c_3 \\&= T(n/8)3c_3 \\&= T(n/16) + c_3 + 3c_3 \\&= T(n/16) + 4c_3 \\&= T(n/32) + c_3 + 4c_3 \\&= T(n/32) + 5c_3\end{aligned}$$

$$T(n/2) = T(n/4) + c_3$$

$$T(n/4) = T(n/8) + c_3$$

$$T(n/8) = T(n/16) + c_3$$

$$T(n/16) = T(n/32) + c_3$$

## 4-19: Solving Recurrence Relations

$$\begin{aligned}T(n) &= T(n/2) + c_3 \\&= T(n/4) + c_3 + c_3 \\&= T(n/4)2c_3 \\&= T(n/8) + c_3 + 2c_3 \\&= T(n/8)3c_3 \\&= T(n/16) + c_3 + 3c_3 \\&= T(n/16) + 4c_3 \\&= T(n/32) + c_3 + 4c_3 \\&= T(n/32) + 5c_3 \\&= \dots \\&= T(n/2^k) + kc_3\end{aligned}$$

$$T(n/2) = T(n/4) + c_3$$

$$T(n/4) = T(n/8) + c_3$$

$$T(n/8) = T(n/16) + c_3$$

$$T(n/16) = T(n/32) + c_3$$

## 4-20: Solving Recurrence Relations

$$T(0) = c_1$$

$$T(1) = c_2$$

$$T(n) = T(n/2) + c_3$$

$$T(n) = T(n/2^k) + kc_3$$

We want to get rid of  $T(n/2^k)$ . We get to a relation we can solve directly when we reach  $T(1)$

$$n/2^k = 1$$

$$n = 2^k$$

$$\lg n = k$$

## 4-21: Solving Recurrence Relations

$$T(0) = c_1$$

$$T(1) = c_2$$

$$T(n) = T(n/2) + c_3$$

$$T(n) = T(n/2^k) + kc_3$$

We want to get rid of  $T(n/2^k)$ . We get to a relation we can solve directly when we reach  $T(1)$

$$\lg n = k$$

$$\begin{aligned} T(n) &= T(n/2^{\lg n}) + \lg n c_3 \\ &= T(1) + c_3 \lg n \\ &= c_2 + c_3 \lg n \\ &\in \Theta(\lg n) \end{aligned}$$

## 4-22: Power *Modifications*

```
long power(long x, long n)
    if (n==0) return 1;
    if (n==1) return x;
    if ((n % 2) == 0)
        return power(x*x, n/2);
    else
        return power(x*x, n/2) * x;
```



## 4-23: Power *Modifications*

```
long power(long x, long n)
    if (n==0) return 1;
    if (n==1) return x;
    if ((n % 2) == 0)
        return power(power(x,2), n/2);
    else
        return power(power(x,2), n/2) * x;
```

This version of power will not work. Why?

## 4-24: Power *Modifications*

```
long power(long x, long n)
    if (n==0) return 1;
    if (n==1) return x;
    if ((n % 2) == 0)
        return power(power(x,n/2), 2);
    else
        return power(power(x,n/2), 2) * x;
```

This version of power also will not work. Why?

## 4-25: Power *Modifications*

```
long power(long x, long n)
    if (n==0) return 1;
    if (n==1) return x;
    if ((n % 2) == 0)
        return power(x,n/2) * power(x,n/2);
    else
        return power(x,n/2) * power(x,n/2) * x;
```

This version of power does work.

What is the recurrence relation that describes its running time?

## 4-26: Power *Modifications*

```
long power(long x, long n)
    if (n==0) return 1;
    if (n==1) return x;
    if ((n % 2) == 0)
        return power(x,n/2) * power(x,n/2);
    else
        return power(x,n.2) * power(x,n/2) * x;
```

$$T(0) = c_1$$

$$T(1) = c_2$$

$$\begin{aligned} T(n) &= T(n/2) + T(n/2) + c_3 \\ &= 2T(n/2) + c_3 \end{aligned}$$

(Again, assume n is a power of 2)

## 4-27: Solving Recurrence Relations

$$\begin{aligned}T(n) &= 2T(n/2) + c_3 \\&= 2[2T(n/4) + c_3]c_3 \\&= 4T(n/4) + 3c_3 \\&= 4[2T(n/8) + c_3] + 3c_3 \\&= 8T(n/8) + 7c_3 \\&= 8[2T(n/16) + c_3] + 7c_3 \\&= 16T(n/16) + 15c_3 \\&= 32T(n/32) + 31c_3 \\&\dots \\&= 2^k T(n/2^k) + (2^k - 1)c_3\end{aligned}$$

$$T(n/2) = 2T(n/4) + c_3$$

$$T(n/4) = 2T(n/8) + c_3$$

## 4-28: Solving Recurrence Relations

$$T(0) = c_1$$

$$T(1) = c_2$$

$$T(n) = 2^k T(n/2^k) + (2^k - 1)c_3$$

Pick a value for  $k$  such that  $n/2^k = 1$ :

$$n/2^k = 1$$

$$n = 2^k$$

$$\lg n = k$$

$$T(n) = 2^{\lg n} T(n/2^{\lg n}) + (2^{\lg n} - 1)c_3$$

$$= nT(n/n) + (n - 1)c_3$$

$$= nT(1) + (n - 1)c_3$$

$$= nc_2 + (n - 1)c_3$$

$$\in \Theta(n)$$